Hacking.

theories/lifetime.v
@@ -1,228 +1,664 @@
-From iris.algebra Require Import csum auth frac gmap.
-From iris.base_logic.lib Require Export fancy_updates invariants namespaces.
+From iris.algebra Require Import csum auth frac gmap dec_agree gset.
+From iris.prelude Require Import gmultiset.
+From iris.base_logic.lib Require Export invariants.
+From iris.base_logic.lib Require Import boxes.
+From iris.base_logic Require Import big_op.
 From iris.proofmode Require Import tactics.
+Import uPred.
 
-Definition lftN := nroot .@ "lft".
+Definition lftN : namespace := nroot .@ "lft".
+Definition borN : namespace := lftN .@ "bor".
+Definition inhN : namespace := lftN .@ "inh".
+Definition mgmtN : namespace := lftN .@ "mgmt".
+
 Definition atomic_lft := positive.
+Notation lft := (gmultiset positive).
+Definition static : lft := ∅.
 
-Definition lft_tokUR : ucmraT :=
-  authUR (gmapUR atomic_lft (csumR fracR unitR)).
+Inductive bor_state :=
+  | Bor_in
+  | Bor_open (q : frac)
+  | Bor_rebor (κ : lft).
+Instance bor_state_eq_dec : EqDecision bor_state.
+Proof. solve_decision. Defined.
 
-(* FIXME : this is not the actual definitions. *)
-Definition borrow_idx := positive.
-Definition borrow_tokUR : ucmraT :=
-  authUR (gmapUR borrow_idx fracR).
+Definition bor_filled (s : bor_state) : bool :=
+  match s with Bor_in => true | _ => false end.
 
-Class lifetimeG Σ := LifetimeG {
-  lft_tok_inG :> inG Σ lft_tokUR;
-  borrow_tok_inG :> inG Σ borrow_tokUR;
-  lft_toks_name : gname;
-  borrow_tok_name : gname
+Definition lft_stateR := csumR fracR unitR.
+Definition to_lft_stateR (b : bool) : lft_stateR :=
+  if b then Cinl 1%Qp else Cinr ().
+
+Record lft_names := LftNames {
+  bor_name : gname;
+  cnt_name : gname;
+  inh_name : gname
+}.
+Instance lft_names_eq_dec : EqDecision lft_names.
+Proof. solve_decision. Defined.
+
+Class lftG Σ := LftG {
+  lft_box :> boxG Σ;
+  lft_atomic_inG :> inG Σ (authR (gmapUR atomic_lft lft_stateR));
+  lft_atomic_name : gname;
+  lft_inter_inG :> inG Σ (authR (gmapUR lft (dec_agreeR lft_names)));
+  lft_inter_name : gname;
+  lft_bor_box :>
+    inG Σ (authR (gmapUR slice_name (prodR fracR (dec_agreeR bor_state))));
+  lft_cnt_inG :> inG Σ (authR natUR);
+  lft_inh_box :> inG Σ (authR (gset_disjUR slice_name));
 }.
 
-Parameter lft_ctx : ∀ `{lifetimeG Σ}, iProp Σ.
-
 Section defs.
+  Context `{invG Σ, lftG Σ}.
 
-  (*** Definitions  *)
+  Definition lft_own (q : Qp) (κ : lft) : iProp Σ :=
+    ([∗ mset] Λ ∈ κ, own lft_atomic_name (◯ {[ Λ := Cinl q ]}))%I.
 
-  Context `{lifetimeG Σ}.
+  Definition lft_dead_own (κ : lft) : iProp Σ :=
+    (∃ Λ, ■ (Λ ∈ κ) ∗ own lft_atomic_name (◯ {[ Λ := Cinr () ]}))%I.
 
-  Definition lifetime := gmap atomic_lft nat.
+  Definition own_lft_auth (I : gmap lft lft_names) : iProp Σ :=
+    own lft_inter_name (● (DecAgree <$> I)).
 
-  Definition static : lifetime := ∅.
+  Definition own_bor (κ : lft)
+      (x : auth (gmap slice_name (frac * dec_agree bor_state))) : iProp Σ :=
+    (∃ γs,
+      own lft_inter_name (◯ {[ κ := DecAgree γs ]}) ∗
+      own (bor_name γs) x)%I.
 
-  Definition Qp_nat_mul  (q : Qp) (n : nat) : option Qp :=
-    match n with
-    | O => None
-    | S n' => Some (Nat.iter n' (λ acc, q ⋅ acc)%Qp q)
-    end.
+  Definition own_cnt (κ : lft) (x : auth nat) : iProp Σ :=
+    (∃ γs,
+      own lft_inter_name (◯ {[ κ := DecAgree γs ]}) ∗
+      own (cnt_name γs) x)%I.
 
-  Definition lft_own (q : Qp) (κ : lifetime) : iProp Σ :=
-    own lft_toks_name (◯ (Cinl <$> omap (Qp_nat_mul q) κ)).
+  Definition own_inh (κ : lft) (x : auth (gset_disj slice_name)) : iProp Σ :=
+    (∃ γs,
+      own lft_inter_name (◯ {[ κ := DecAgree γs ]}) ∗
+      own (inh_name γs) x)%I.
 
-  Definition lft_dead (κ : lifetime) : iProp Σ :=
-    (∃ Λ, ■ (∃ n, κ !! Λ = Some (S n)) ∗
-            own lft_toks_name (◯ {[ Λ := Cinr () ]}))%I.
+  Definition bor_cnt (κ : lft) (s : bor_state) : iProp Σ :=
+    match s with
+    | Bor_in => True
+    | Bor_open q => lft_own q κ
+    | Bor_rebor κ' => ■ (κ ⊂ κ') ∗ own_cnt κ' (◯ 1)
+    end%I.
 
-  Definition idx_borrow_own (q : Qp) (i : borrow_idx) :=
-    own borrow_tok_name (◯ {[ i := q ]}).
+  Definition lft_bor_alive (κ : lft) (P : iProp Σ) : iProp Σ :=
+    (∃ B : gmap slice_name bor_state,
+      box borN (bor_filled <$> B) P ∗
+      own_bor κ (● ((1%Qp,) ∘ DecAgree <$> B)) ∗
+      [∗ map] s ∈ B, bor_cnt κ s)%I.
 
-  Parameter idx_borrow:
-    ∀ `{lifetimeG Σ} (κ : lifetime) (i : borrow_idx) (P : iProp Σ), iProp Σ.
+  Definition lft_bor_dead (κ : lft) : iProp Σ :=
+     (∃ (B: gset slice_name) (P : iProp Σ),
+       own_bor κ (● to_gmap (1%Qp, DecAgree Bor_in) B) ∗
+       box borN (to_gmap false B) P)%I.
 
-  Definition borrow (κ : lifetime) (P : iProp Σ) : iProp Σ :=
-    (∃ i, idx_borrow κ i P ∗ idx_borrow_own 1 i)%I.
+   Definition lft_inh (κ : lft) (s : bool) (P : iProp Σ) : iProp Σ :=
+     (∃ E : gset slice_name,
+       own_inh κ (● GSet E) ∗
+       box inhN (to_gmap s E) P)%I.
 
+   Definition lft_vs_inv_go (κ : lft) (lft_alive : ∀ κ', κ' ⊂ κ → iProp Σ)
+       (I : gmap lft lft_names) : iProp Σ :=
+     (lft_bor_dead κ ∗
+       own_lft_auth I ∗
+       [∗ set] κ' ∈ dom _ I, ∀ Hκ : κ' ⊂ κ, lft_alive κ' Hκ)%I.
+
+   Definition lft_vs_go (κ : lft) (lft_alive : ∀ κ', κ' ⊂ κ → iProp Σ)
+       (P Q : iProp Σ) : iProp Σ :=
+     (∃ n : nat,
+       own_cnt κ (● n) ∗
+       ∀ I : gmap lft lft_names,
+         lft_vs_inv_go κ lft_alive I -∗ ▷ P -∗ lft_dead_own κ
+           ={⊤∖nclose mgmtN}=∗
+         lft_vs_inv_go κ lft_alive I ∗ ▷ Q ∗ own_cnt κ (◯ n))%I.
+
+  Definition lft_alive_go (κ : lft) (lft_alive : ∀ κ', κ' ⊂ κ → iProp Σ) : iProp Σ :=
+    (∃ P Q,
+      lft_bor_alive κ P ∗
+      lft_vs_go κ lft_alive P Q ∗
+      lft_inh κ false Q)%I.
+
+  Definition lft_alive (κ : lft) : iProp Σ :=
+    Fix_F _ lft_alive_go (gmultiset_wf κ).
+  Definition lft_vs_inv (κ : lft) (I : gmap lft lft_names) : iProp Σ :=
+    lft_vs_inv_go κ (λ κ' _, lft_alive κ') I.
+  Definition lft_vs (κ : lft) (P Q : iProp Σ) : iProp Σ :=
+    lft_vs_go κ (λ κ' _, lft_alive κ') P Q.
+
+  Definition lft_dead (κ : lft) : iProp Σ :=
+    (∃ P,
+      lft_bor_dead κ ∗
+      own_cnt κ (● 0) ∗
+      lft_inh κ true P)%I.
+
+  Definition lft_inv (A : gmap atomic_lft bool) (κ : lft) : iProp Σ :=
+    ((lft_alive κ ∗ ■ ∀ Λ, Λ ∈ κ → A !! Λ = Some true)
+    ∨ (lft_dead κ ∗ ■ ∃ Λ, Λ ∈ κ ∧ A !! Λ = Some false))%I.
+
+  Definition lfts_inv : iProp Σ :=
+    (∃ (A : gmap atomic_lft bool) (I : gmap lft lft_names),
+      own lft_atomic_name (● (to_lft_stateR <$> A)) ∗
+      own_lft_auth I ∗
+      [∗ set] κ ∈ dom _ I, lft_inv A κ)%I.
+
+  Definition lft_ctx : iProp Σ := inv mgmtN lfts_inv.
+
+  Definition lft_incl (κ κ' : lft) : iProp Σ :=
+    (□ ((∀ q, lft_own q κ ={lftN}=∗ ∃ q',
+                 lft_own q' κ' ∗ (lft_own q' κ' ={lftN}=∗ lft_own q κ)) ∗
+        (lft_dead_own κ' ={lftN}=∗ lft_dead_own κ)))%I.
+
+  Definition bor_idx := (lft * slice_name)%type.
+
+  Definition idx_bor_own (q : frac) (i : bor_idx) : iProp Σ :=
+    own_bor (i.1) (◯ {[ i.2 := (q,DecAgree Bor_in) ]}).
+  Definition idx_bor (κ : lft) (i : bor_idx) (P : iProp Σ) : iProp Σ :=
+    (lft_incl κ (i.1) ∗ slice borN (i.2) P)%I.
+  Definition raw_bor (i : bor_idx) (P : iProp Σ) : iProp Σ :=
+    (idx_bor_own 1 i ∗ slice borN (i.2) P)%I.
+  Definition bor (κ : lft) (P : iProp Σ) : iProp Σ :=
+    (∃ i, lft_incl κ (i.1) ∗ raw_bor i P)%I.
 End defs.
 
-Typeclasses Opaque lft_own lft_dead borrow.
-
-(*** Notations  *)
+Instance: Params (@lft_bor_alive) 4.
+Instance: Params (@lft_inh) 5.
+Instance: Params (@lft_vs) 4.
+Instance: Params (@idx_bor) 5.
+Instance: Params (@raw_bor) 4.
+Instance: Params (@bor) 4.
 
 Notation "q .[ κ ]" := (lft_own q κ)
-    (format "q .[ κ ]", at level 0): uPred_scope.
-Notation "[† κ ]" := (lft_dead κ) (format "[† κ ]"): uPred_scope.
-Notation "&{ κ } P" := (borrow κ P)
-  (format "&{ κ } P", at level 20, right associativity) : uPred_scope.
-Hint Unfold lifetime : typeclass_instances.
+    (format "q .[ κ ]", at level 0) : uPred_scope.
+Notation "[† κ ]" := (lft_dead_own κ) (format "[† κ ]"): uPred_scope.
 
-Section lft.
-  Context `{invG Σ, lifetimeG Σ}.
+Notation "&{ κ } P" := (bor κ P)
+  (format "&{ κ }  P", at level 20, right associativity) : uPred_scope.
+Notation "&{ κ , i } P" := (idx_bor κ i P)
+  (format "&{ κ , i }  P", at level 20, right associativity) : uPred_scope.
 
-  Axiom lft_ctx_alloc : True ={∅}=∗ lft_ctx.
+Infix "⊑" := lft_incl (at level 70) : uPred_scope.
 
-  (*** PersitentP, TimelessP and Proper instances  *)
+(*
+Typeclasses Opaque lft_own lft_dead borrow.
+*)
 
-  Global Instance lft_own_timeless q κ : TimelessP q.[κ].
-  Proof. unfold lft_own. apply _. Qed.
+Section theorems.
+Context `{invG Σ, lftG Σ}.
+Implicit Types κ : lft.
 
-  Global Instance lft_dead_persistent κ : PersistentP [†κ].
-  Proof. unfold lft_dead. apply _. Qed.
-  Global Instance lft_dead_timeless κ : PersistentP [†κ].
-  Proof. unfold lft_dead. apply _. Qed.
+(* Unfolding lemmas *)
+Lemma lft_vs_inv_go_ne κ (f f' : ∀ κ', κ' ⊂ κ → iProp Σ) I n :
+  (∀ κ' (Hκ : κ' ⊂ κ), f κ' Hκ ≡{n}≡ f' κ' Hκ) →
+  lft_vs_inv_go κ f I ≡{n}≡ lft_vs_inv_go κ f' I.
+Proof.
+  intros Hf. apply sep_ne, sep_ne, big_opS_ne=> // κ'.
+  by apply forall_ne=> Hκ.
+Qed.
 
-  Axiom idx_borrow_persistent :
-    ∀ κ i P, PersistentP (idx_borrow κ i P).
-  Global Existing Instance idx_borrow_persistent.
-  Axiom idx_borrow_proper :
-    ∀ κ i, Proper ((⊣⊢) ==> (⊣⊢)) (idx_borrow κ i).
-  Global Existing Instance idx_borrow_proper.
+Lemma lft_vs_go_ne κ (f f' : ∀ κ', κ' ⊂ κ → iProp Σ) P P' Q Q' n :
+  (∀ κ' (Hκ : κ' ⊂ κ), f κ' Hκ ≡{n}≡ f' κ' Hκ) →
+  P ≡{n}≡ P' → Q ≡{n}≡ Q' →
+  lft_vs_go κ f P Q ≡{n}≡ lft_vs_go κ f' P' Q'.
+Proof.
+  intros Hf HP HQ. apply exist_ne=> n'.
+  apply sep_ne, forall_ne=> // I. rewrite lft_vs_inv_go_ne //. solve_proper.
+Qed.
 
-  Axiom idx_borrow_own_timeless :
-    ∀ q i, TimelessP (idx_borrow_own q i).
-  Global Existing Instance idx_borrow_own_timeless.
+Lemma lft_alive_go_ne κ (f f' : ∀ κ', κ' ⊂ κ → iProp Σ) n :
+  (∀ κ' (Hκ : κ' ⊂ κ), f κ' Hκ ≡{n}≡ f' κ' Hκ) →
+  lft_alive_go κ f ≡{n}≡ lft_alive_go κ f'.
+Proof.
+  intros Hf. apply exist_ne=> P; apply exist_ne=> Q. by rewrite lft_vs_go_ne.
+Qed.
 
-  Global Instance borrow_proper κ: Proper ((⊣⊢) ==> (⊣⊢)) (borrow κ).
-  Proof. solve_proper. Qed.
+Lemma lft_alive_unfold κ :
+  lft_alive κ ⊣⊢ ∃ P Q, lft_bor_alive κ P ∗ lft_vs κ P Q ∗ lft_inh κ false Q.
+Proof.
+  apply equiv_dist=> n. rewrite /lft_alive -Fix_F_eq.
+  apply lft_alive_go_ne=> κ' Hκ.
+  apply (Fix_F_proper _ (λ _, dist n)); auto using lft_alive_go_ne.
+Qed.
+Lemma lft_vs_inv_unfold κ (I : gmap lft lft_names) :
+  lft_vs_inv κ I ⊣⊢ lft_bor_dead κ ∗
+    own_lft_auth I ∗
+    [∗ set] κ' ∈ dom _ I, ■ (κ' ⊂ κ) → lft_alive κ'.
+Proof.
+  rewrite /lft_vs_inv /lft_vs_inv_go. by setoid_rewrite pure_impl_forall.
+Qed.
+Lemma lft_vs_unfold κ P Q :
+  lft_vs κ P Q ⊣⊢ ∃ n : nat,
+    own_cnt κ (● n) ∗
+    ∀ I : gmap lft lft_names,
+      lft_vs_inv κ I -∗ ▷ P -∗ lft_dead_own κ ={⊤∖nclose mgmtN}=∗
+      lft_vs_inv κ I ∗ ▷ Q ∗ own_cnt κ (◯ n).
+Proof. done. Qed.
 
-  Axiom lft_ctx_persistent : PersistentP lft_ctx.
+Global Instance lft_bor_alive_ne κ n : Proper (dist n ==> dist n) (lft_bor_alive κ).
+Proof. solve_proper. Qed.
+Global Instance lft_bor_alive_proper κ : Proper ((≡) ==> (≡)) (lft_bor_alive κ).
+Proof. apply (ne_proper _). Qed.
 
-  (** Basic rules about lifetimes  *)
-  Lemma lft_own_op q κ1 κ2 : q.[κ1] ∗ q.[κ2] ⊣⊢ q.[κ1 ⋅ κ2].
-  Proof.
-    rewrite /lft_own -own_op. f_equiv. constructor. done. move=>Λ /=.
-    rewrite lookup_op !lookup_fmap !lookup_omap lookup_op.
-    case: (κ1 !! Λ)=>[[|a1]|]; case: (κ2 !! Λ)=>[[|a2]|]/=; rewrite ?right_id ?left_id //.
-    apply reflexive_eq. apply (f_equal (Some ∘ Cinl)).
-    induction a1. done. rewrite /= -assoc. by f_equal.
-  Qed.
+Global Instance lft_inh_ne κ s n : Proper (dist n ==> dist n) (lft_inh κ s).
+Proof. solve_proper. Qed.
+Global Instance lft_inh_proper κ s : Proper ((≡) ==> (≡)) (lft_inh κ s).
+Proof. apply (ne_proper _). Qed.
 
-  Lemma lft_dead_or κ1 κ2 : [†κ1] ∨ [†κ2] ⊣⊢ [† κ1⋅κ2].
-  Proof.
-    unfold lft_dead. setoid_rewrite lookup_op. iSplit.
-    - iIntros "[H|H]"; iDestruct "H" as (Λ) "[H?]";
-        iDestruct "H" as %[n Hn]; iExists _; iFrame; iPureIntro; rewrite Hn.
-      + case: (κ2 !! Λ); eauto.
-      + case: (κ1 !! Λ)=>[n'|]; eauto. exists (n' + n)%nat. by apply (f_equal Some).
-    - iIntros "H". iDestruct "H" as (Λ) "[H Hown]"; eauto. iDestruct "H" as %[n Hn].
-      case K1: (κ1 !! Λ) Hn=>[[|a1]|]; case K2: (κ2 !! Λ)=>[[|a2]|]; intros [=<-];
-      (iRight + iLeft); iExists Λ; iIntros "{$Hown}!%"; by eauto.
-  Qed.
+Global Instance lft_vs_ne κ n :
+  Proper (dist n ==> dist n ==> dist n) (lft_vs κ).
+Proof. intros P P' HP Q Q' HQ. by apply lft_vs_go_ne. Qed.
+Global Instance lft_vs_proper κ : Proper ((≡) ==> (≡) ==> (≡)) (lft_vs κ).
+Proof. apply (ne_proper_2 _). Qed.
 
-  Lemma lft_own_frac_op κ q q':
-       (q + q').[κ] ⊣⊢ q.[κ] ∗ q'.[κ].
-  Proof.
-    rewrite /lft_own -own_op -auth_frag_op. f_equiv. constructor. done. simpl.
-    intros Λ. rewrite lookup_op !lookup_fmap !lookup_omap. apply reflexive_eq.
-    case: (κ !! Λ)=>[[|a]|]//=. rewrite -Some_op Cinl_op. repeat f_equal.
-    induction a as [|a IH]. done.
-    rewrite /= IH /op /cmra_op /= /frac_op !assoc. f_equal.
-    rewrite -!assoc. f_equal. apply (comm _).
-  Qed.
+Global Instance idx_bor_ne κ i n : Proper (dist n ==> dist n) (idx_bor κ i).
+Proof. solve_proper. Qed.
+Global Instance idx_bor_proper κ i : Proper ((≡) ==> (≡)) (idx_bor κ i).
+Proof. apply (ne_proper _). Qed.
 
-  Axiom lft_create :
-    ∀ `(nclose lftN ⊆ E),
-      lft_ctx ={E}=∗ ∃ κ, 1.[κ] ∗ □ (1.[κ] ={⊤,⊤∖nclose lftN}▷=∗ [†κ]).
+Global Instance raw_bor_ne i n : Proper (dist n ==> dist n) (raw_bor i).
+Proof. solve_proper. Qed.
+Global Instance raw_bor_proper i : Proper ((≡) ==> (≡)) (raw_bor i).
+Proof. apply (ne_proper _). Qed.
 
-  Axiom idx_borrow_acc :
-    ∀ `(nclose lftN ⊆ E) q κ i P,
-      lft_ctx ⊢ idx_borrow κ i P -∗ idx_borrow_own 1 i
-              -∗ q.[κ] ={E}=∗ ▷ P ∗ (▷ P ={E}=∗ idx_borrow_own 1 i ∗ q.[κ]).
-  Axiom idx_borrow_atomic_acc :
-    ∀ `(nclose lftN ⊆ E) q κ i P,
-      lft_ctx ⊢ idx_borrow κ i P -∗ idx_borrow_own q i
-         ={E,E∖lftN}=∗
-            ▷ P ∗ (▷ P ={E∖lftN,E}=∗ idx_borrow_own q i) ∨
-            [†κ] ∗ (|={E∖lftN,E}=> idx_borrow_own q i).
+Global Instance bor_ne κ n : Proper (dist n ==> dist n) (bor κ).
+Proof. solve_proper. Qed.
+Global Instance bor_proper κ : Proper ((≡) ==> (≡)) (bor κ).
+Proof. apply (ne_proper _). Qed.
 
-  (** Basic borrows  *)
-  Axiom borrow_create :
-    ∀ `(nclose lftN ⊆ E) κ P, lft_ctx ⊢ ▷ P ={E}=∗ &{κ} P ∗ ([†κ] ={E}=∗ ▷ P).
-  Axiom borrow_fake : ∀ `(nclose lftN ⊆ E) κ P, lft_ctx ⊢ [†κ] ={E}=∗ &{κ}P.
-  Axiom borrow_split :
-    ∀ `(nclose lftN ⊆ E) κ P Q, lft_ctx ⊢ &{κ}(P ∗ Q) ={E}=∗ &{κ}P ∗ &{κ}Q.
-  Axiom borrow_combine :
-    ∀ `(nclose lftN ⊆ E) κ P Q, lft_ctx ⊢ &{κ}P -∗ &{κ}Q ={E}=∗ &{κ}(P ∗ Q).
-  Axiom borrow_acc_strong :
-    ∀ `(nclose lftN ⊆ E) q κ P,
-      lft_ctx ⊢ &{κ}P -∗ q.[κ] ={E}=∗ ▷ P ∗
-      ∀ Q, ▷ Q ∗ ▷([†κ] -∗ ▷Q ={⊤ ∖ nclose lftN}=∗ ▷ P) ={E}=∗ &{κ}Q ∗ q.[κ].
-  Axiom borrow_acc_atomic_strong :
-    ∀ `(nclose lftN ⊆ E) κ P,
-      lft_ctx ⊢ &{κ}P ={E,E∖lftN}=∗
-        (▷ P ∗ ∀ Q, ▷ Q ∗ ▷([†κ] -∗ ▷Q ={⊤ ∖ nclose lftN}=∗ ▷ P) ={E∖lftN,E}=∗ &{κ}Q) ∨
-        [†κ] ∗ |={E∖lftN,E}=> True.
-  Axiom borrow_reborrow' :
-    ∀ `(nclose lftN ⊆ E) κ κ' P, κ ≼ κ' →
-      lft_ctx ⊢ &{κ}P ={E}=∗ &{κ'}P ∗ ([†κ'] ={E}=∗ &{κ}P).
-  Axiom borrow_unnest :
-    ∀ `(nclose lftN ⊆ E) κ κ' P, lft_ctx ⊢ &{κ'}&{κ}P ={E}▷=∗ &{κ ⋅ κ'}P.
+(*** PersistentP and TimelessP instances  *)
+Global Instance lft_own_timeless q κ : TimelessP q.[κ].
+Proof. rewrite /lft_own. apply _. Qed.
+Global Instance lft_dead_own_persistent κ : PersistentP [†κ].
+Proof. rewrite /lft_own. apply _. Qed.
+Global Instance lft_dead_own_timeless κ : PersistentP [†κ].
+Proof. rewrite /lft_own. apply _. Qed.
+
+Global Instance idx_bor_persistent κ i P : PersistentP (&{κ,i} P).
+Proof. rewrite /idx_bor. apply _. Qed.
+Global Instance idx_borrow_own_timeless q i : TimelessP (idx_bor_own q i).
+Proof. rewrite /idx_bor_own. apply _. Qed.
+
+Global Instance lft_incl_persistent κ κ' : PersistentP (κ ⊑ κ').
+Proof. apply _. Qed.
+Global Instance lft_ctx_persistent : PersistentP lft_ctx.
+Proof. apply _. Qed.
+
+(** Silly stuff *)
+Lemma foo (I : gmap lft lft_names) κ γs :
+  own_lft_auth I ⊢
+    own lft_inter_name (◯ {[κ := DecAgree γs]}) -∗ ■ is_Some (I !! κ).
+Proof.
+  iIntros "HI Hκ". iDestruct (own_valid_2 with "HI Hκ")
+    as %[[? [??]]%singleton_included _]%auth_valid_discrete_2.
+  simplify_map_eq; simplify_option_eq; eauto.
+Qed.
+
+Lemma own_bor_auth I κ x : own_lft_auth I ⊢ own_bor κ x -∗ ■ is_Some (I !! κ).
+Proof. iIntros "HI"; iDestruct 1 as (γs) "[? _]". by iApply (foo with "HI"). Qed.
+Lemma own_bor_op κ x y : own_bor κ (x ⋅ y) ⊣⊢ own_bor κ x ∗ own_bor κ y.
+Proof.
+  iSplit.
+  { iDestruct 1 as (γs) "[#? [Hx Hy]]"; iSplitL "Hx"; iExists γs; eauto. }
+  iIntros "[Hx Hy]".
+  iDestruct "Hx" as (γs) "[Hγs Hx]"; iDestruct "Hy" as (γs') "[Hγs' Hy]".
+  iDestruct (own_valid_2 with "Hγs Hγs'") as %Hγs%auth_own_valid.
+  move: Hγs; rewrite /= op_singleton singleton_valid=> /dec_agree_op_inv [<-].
+  iExists γs. iSplit. done. rewrite own_op; iFrame.
+Qed.
+Lemma own_bor_valid κ x : own_bor κ x ⊢ ✓ x.
+Proof. iDestruct 1 as (γs) "[#? Hx]". by iApply own_valid. Qed.
+Lemma own_bor_valid_2 κ x y : own_bor κ x ⊢ own_bor κ y -∗ ✓ (x ⋅ y).
+Proof. apply wand_intro_r. rewrite -own_bor_op. apply own_bor_valid. Qed.
+Lemma own_bor_update κ x y : x ~~> y → own_bor κ x ==∗ own_bor κ y.
+Proof.
+  iDestruct 1 as (γs) "[#Hκ Hx]"; iExists γs. iFrame "Hκ". by iApply own_update.
+Qed.
+
+Lemma own_cnt_auth I κ x : own_lft_auth I ⊢ own_cnt κ x -∗ ■ is_Some (I !! κ).
+Proof. iIntros "HI"; iDestruct 1 as (γs) "[? _]". by iApply (foo with "HI"). Qed.
+Lemma own_cnt_op κ x y : own_cnt κ (x ⋅ y) ⊣⊢ own_cnt κ x ∗ own_cnt κ y.
+Proof.
+  iSplit.
+  { iDestruct 1 as (γs) "[#? [Hx Hy]]"; iSplitL "Hx"; iExists γs; eauto. }
+  iIntros "[Hx Hy]".
+  iDestruct "Hx" as (γs) "[Hγs Hx]"; iDestruct "Hy" as (γs') "[Hγs' Hy]".
+  iDestruct (own_valid_2 with "Hγs Hγs'") as %Hγs%auth_own_valid.
+  move: Hγs; rewrite /= op_singleton singleton_valid=> /dec_agree_op_inv [<-].
+  iExists γs. iSplit. done. rewrite own_op; iFrame.
+Qed.
+Lemma own_cnt_valid κ x : own_cnt κ x ⊢ ✓ x.
+Proof. iDestruct 1 as (γs) "[#? Hx]". by iApply own_valid. Qed.
+Lemma own_cnt_valid_2 κ x y : own_cnt κ x ⊢ own_cnt κ y -∗ ✓ (x ⋅ y).
+Proof. apply wand_intro_r. rewrite -own_cnt_op. apply own_cnt_valid. Qed.
+Lemma own_cnt_update κ x y : x ~~> y → own_cnt κ x ==∗ own_cnt κ y.
+Proof.
+  iDestruct 1 as (γs) "[#Hκ Hx]"; iExists γs. iFrame "Hκ". by iApply own_update.
+Qed.
+Lemma own_cnt_update_2 κ x1 x2 y :
+  x1 ⋅ x2 ~~> y → own_cnt κ x1 ⊢ own_cnt κ x2 ==∗ own_cnt κ y.
+Proof.
+  intros. apply wand_intro_r. rewrite -own_cnt_op. by apply own_cnt_update.
+Qed.
+
+Lemma own_inh_auth I κ x : own_lft_auth I ⊢ own_inh κ x -∗ ■ is_Some (I !! κ).
+Proof. iIntros "HI"; iDestruct 1 as (γs) "[? _]". by iApply (foo with "HI"). Qed.
+Lemma own_inh_op κ x y : own_inh κ (x ⋅ y) ⊣⊢ own_inh κ x ∗ own_inh κ y.
+Proof.
+  iSplit.
+  { iDestruct 1 as (γs) "[#? [Hx Hy]]"; iSplitL "Hx"; iExists γs; eauto. }
+  iIntros "[Hx Hy]".
+  iDestruct "Hx" as (γs) "[Hγs Hx]"; iDestruct "Hy" as (γs') "[Hγs' Hy]".
+  iDestruct (own_valid_2 with "Hγs Hγs'") as %Hγs%auth_own_valid.
+  move: Hγs; rewrite /= op_singleton singleton_valid=> /dec_agree_op_inv [<-].
+  iExists γs. iSplit. done. rewrite own_op; iFrame.
+Qed.
+Lemma own_inh_valid κ x : own_inh κ x ⊢ ✓ x.
+Proof. iDestruct 1 as (γs) "[#? Hx]". by iApply own_valid. Qed.
+Lemma own_inh_valid_2 κ x y : own_inh κ x ⊢ own_inh κ y -∗ ✓ (x ⋅ y).
+Proof. apply wand_intro_r. rewrite -own_inh_op. apply own_inh_valid. Qed.
+Lemma own_inh_update κ x y : x ~~> y → own_inh κ x ==∗ own_inh κ y.
+Proof.
+  iDestruct 1 as (γs) "[#Hκ Hx]"; iExists γs. iFrame "Hκ". by iApply own_update.
+Qed.
+
+(** Basic rules about lifetimes  *)
+Lemma lft_own_op q κ1 κ2 : q.[κ1] ∗ q.[κ2] ⊣⊢ q.[κ1 ∪ κ2].
+Proof. by rewrite /lft_own -big_sepMS_union. Qed.
+
+Lemma lft_dead_own_or κ1 κ2 : [†κ1] ∨ [†κ2] ⊣⊢ [† κ1 ∪ κ2].
+Proof.
+  rewrite /lft_dead_own -or_exist. apply exist_proper=> Λ.
+  rewrite -sep_or_r -pure_or. do 2 f_equiv. set_solver.
+Qed.
+
+Lemma lft_own_frac_op κ q q' : (q + q').[κ] ⊣⊢ q.[κ] ∗ q'.[κ].
+Proof.
+  rewrite /lft_own -big_sepMS_sepMS. apply big_sepMS_proper=> Λ _.
+  by rewrite -own_op -auth_frag_op op_singleton.
+Qed.
+
+Lemma lft_own_split κ q : q.[κ] ⊣⊢ (q/2).[κ] ∗ (q/2).[κ].
+Proof. by rewrite -lft_own_frac_op Qp_div_2. Qed.
+
+Lemma lft_own_dead_own q κ : q.[κ] ⊢ [† κ] -∗ False.
+Proof.
+  rewrite /lft_own /lft_dead_own. iIntros "H"; iDestruct 1 as (Λ') "[% H']".
+  iDestruct (big_sepMS_elem_of _ _ Λ' with "H") as "H"=> //.
+  iDestruct (own_valid_2 with "H H'") as %Hvalid.
+  move: Hvalid=> /auth_own_valid /=; by rewrite op_singleton singleton_valid.
+Qed.
+
+Lemma lft_own_static q : True ⊢ q.[static].
+Proof. by rewrite /lft_own big_sepMS_empty. Qed.
+
+Lemma lft_own_dead_static : [† static] ⊢ False.
+Proof. iDestruct 1 as (Λ) "[% H']". set_solver. Qed.
+
+(* Lifetime creation *)
+Lemma lft_inh_kill E κ Q :
+  nclose inhN ⊆ E →
+  lft_inh κ false Q ∗ ▷ Q ={E}=∗ lft_inh κ true Q.
+Proof.
+  iIntros (?) "[Hinh HQ]". iDestruct "Hinh" as (E') "[Hinh Hbox]".
+  iMod (box_fill_all with "[$Hbox $HQ]") as "?"=>//.
+  rewrite fmap_to_gmap. iModIntro. iExists E'. by iFrame.
+Qed.
+
+Lemma lft_vs_inv_frame (KI K : gset lft) κ :
+  (∀ κ', κ' ∈ KI → κ' ⊂ κ → κ' ∈ K) →
+  ([∗ set] κ' ∈ K, lft_alive κ') ⊢
+    ([∗ set] κ' ∈ KI, ■ (κ' ⊂ κ) → lft_alive κ') ∗
+    (([∗ set] κ' ∈ KI, ■ (κ' ⊂ κ) → lft_alive κ') -∗
+      ([∗ set] κ' ∈ K, lft_alive κ')).
+Proof.
+  intros ?.
+  destruct (proj1 (subseteq_disjoint_union_L (filter (⊂ κ) KI) K)) as (K'&->&?).
+  { intros κ'. rewrite elem_of_filter. set_solver. }
+  rewrite big_sepS_union // big_sepS_filter. iIntros "[$ $]"; auto.
+Qed.
+
+Lemma ilft_create A I κ :
+  own_lft_auth I ⊢ ([∗ set] κ ∈ dom _ I, lft_inv A κ)
+      ==∗ ∃ I', ■ (is_Some (I' !! κ)) ∗
+    own_lft_auth I' ∗ ([∗ set] κ ∈ dom _ I', lft_inv A κ).
+Proof.
+  iIntros "HI HA".
+  destruct (decide (is_Some (I !! κ))) as [?|HIκ%eq_None_not_Some].
+  { iModIntro. iExists I. by iFrame. }
+  iMod (own_alloc (● 0)) as (γcnt) "Hcnt"; first done.
+  iMod (own_alloc ((● ∅ ⋅ ◯ ∅) :auth (gmap slice_name
+      (frac * dec_agree bor_state)))) as (γbor) "[Hbor Hbor']";
+    first by apply auth_valid_discrete_2.
+  iMod (own_alloc ((● ∅ ⋅ ◯ ∅) :auth (gset_disj slice_name)))
+    as (γinh) "[Hinh Hinh']"; first by apply auth_valid_discrete_2.
+  set (γs := LftNames γbor γcnt γinh).
+  iMod (own_update with "HI") as "[HI Hγs]".
+  { apply auth_update_alloc,
+      (alloc_singleton_local_update _ κ (DecAgree γs)); last done.
+    by rewrite lookup_fmap HIκ. }
+  iModIntro. iExists (<[κ:=γs]> I).
+  iSplit; first rewrite lookup_insert; eauto.
+  iSplitL "HI"; first by rewrite /own_lft_auth fmap_insert.
+  rewrite dom_insert_L big_sepS_insert ?not_elem_of_dom //. iFrame "HA".
+  rewrite /lft_inv.
+  destruct (decide (set_Exists (λ Λ, A !! Λ = Some false)
+    (dom (gset _) κ))) as [(Λ & HΛ%gmultiset_elem_of_dom & ?)|?].
+  - iRight. iSplitL; last by eauto.
+    admit.
+  - iLeft. iSplitL. admit.
+Admitted.
+
+Lemma lft_kill (I : gmap lft lft_names) (K K' : gset lft) (κ : lft) :
+  let Iinv := (
+    own_lft_auth I ∗
+    ([∗ set] κ' ∈ K, lft_alive κ') ∗
+    ([∗ set] κ' ∈ K', lft_dead κ'))%I in
+  (∀ κ', is_Some (I !! κ') → κ' ⊂ κ → κ' ∈ K) →
+  (∀ κ', is_Some (I !! κ') → κ ⊂ κ' → κ' ∈ K') →
+  Iinv ⊢ lft_alive κ -∗ [†κ] ={⊤∖nclose mgmtN}=∗ Iinv ∗ lft_dead κ.
+Proof.
+  iIntros (Iinv HK HK') "(HI & Halive & Hdead) Hlalive Hκ".
+  rewrite lft_alive_unfold; iDestruct "Hlalive" as (P Q) "(Hbor & Hvs & Hinh)".
+  iDestruct "Hbor" as (B) "(Hbox & Hbor & HB)".
+  iAssert (■ ∀ i s, B !! i = Some s → s = Bor_in)%I with "[#]" as %HB.
+  { iIntros (i s HBI).
+    iDestruct (big_sepM_lookup _ B with "HB") as "HB"=> //.
+    destruct s as [|q|κ']; rewrite /bor_cnt //.
+    { iDestruct (lft_own_dead_own with "HB Hκ") as "[]". }
+    iDestruct "HB" as "[% Hcnt]".
+    iDestruct (own_cnt_auth with "HI Hcnt") as %?.
+    iDestruct (big_sepS_elem_of _ K' with "Hdead") as "Hdead"; first by eauto.
+    iDestruct "Hdead" as (R) "(_ & Hcnt' & _)".
+    iDestruct (own_cnt_valid_2 with "Hcnt' Hcnt")
+      as %[?%nat_included _]%auth_valid_discrete_2; omega. }
+  iMod (box_empty_all with "Hbox") as "[HP Hbox]"=>//; first solve_ndisj.
+  { intros i s. by rewrite lookup_fmap fmap_Some=> -[? [/HB -> ->]]. }
+  rewrite lft_vs_unfold; iDestruct "Hvs" as (n) "[Hcnt Hvs]".
+  iDestruct (lft_vs_inv_frame (dom _ I) _ κ with "Halive") as "[Halive Halive']".
+  { intros κ'. rewrite elem_of_dom. eauto. }
+  iMod ("Hvs" $! I with "[HI Halive Hbox Hbor] HP Hκ") as "(Hinv & HQ & Hcnt')".
+  { rewrite lft_vs_inv_unfold. iFrame. iExists (dom _ B), P.
+    rewrite !to_gmap_dom -map_fmap_compose.
+    rewrite (map_fmap_ext _ ((1%Qp,) ∘ DecAgree) B); last naive_solver.
+    iFrame. }
+  rewrite lft_vs_inv_unfold; iDestruct "Hinv" as "(?&HI&Halive)".
+  iSpecialize ("Halive'" with "Halive").
+  iMod (own_cnt_update_2 with "Hcnt Hcnt'") as "?".
+  { apply auth_update_dealloc, (nat_local_update _ _ 0 0); omega. }
+  rewrite /Iinv. iFrame "Hdead Halive' HI".
+  iMod (lft_inh_kill with "[$Hinh $HQ]"); first solve_ndisj.
+  iModIntro. iExists Q. by iFrame.
+Qed.
+
+Lemma lfts_kill (I : gmap lft lft_names) (K K' : gset lft) :
+  let Iinv K' := (own_lft_auth I ∗ ([∗ set] κ' ∈ K', lft_alive κ'))%I in
+  (∀ κ, κ ∈ K → is_Some (I !! κ)) →
+  K ⊥ K' →
+  (∀ κ κ', κ ∈ K → is_Some (I !! κ') → κ ⊆ κ' → κ' ∈ K) →
+  (∀ κ κ', is_Some (I !! κ') → κ' ∉ K → κ ∈ K → κ' ⊂ κ → κ' ∈ K') →
+  Iinv K' ⊢ ([∗ set] κ ∈ K, lft_alive κ ∗ [†κ])
+    ={⊤∖nclose mgmtN}=∗ Iinv K' ∗ [∗ set] κ ∈ K, lft_dead κ.
+Proof.
+  intros Iinv. revert K'.
+  induction (collection_wf K) as [K _ IH]=> K' HIK HKK' HK HK'.
+  iIntros "[HI Halive] HK". destruct (decide (K = ∅)) as [->|].
+  { iModIntro. rewrite /Iinv. iFrame. by iApply (big_sepS_empty lft_dead). }
+  destruct (minimal_exists_L (⊂) K) as (κ & HκK & Hκmin); first done.
+  iDestruct (big_sepS_delete _ K with "HK") as "[[Hκalive Hκ] HK]"; first done.
+  destruct (HIK κ) as [γs Hκ]; first done.
+  specialize (IH (K ∖ {[ κ ]})). feed specialize IH.
+  { clear IH. set_unfold. (* HERE *)
+assert (LeibnizEquiv (option ())). apply _.
+Typeclasses eauto := debug.
+ set_unfold. naive_solver. set_solver. clear -HκK. set_solver. SearchAbout strict difference. abstract set_solver +HκK. }
+  assert (κ ∉ K') by set_solver +HKK' HκK.
+  iMod (IH ({[ κ ]} ∪ K') with "[HI Halive Hκalive] HK") as "[[HI Halive] Hdead]".
+  { intros κ' [? _]%elem_of_difference; eauto. }
+  { intros κ'. rewrite elem_of_difference elem_of_union !elem_of_singleton.
+    naive_solver. }
+  { intros κ' κ''. rewrite -> minimal_strict in Hκmin.
+    rewrite !elem_of_difference !elem_of_singleton=> -[? Hneq] ??; split; eauto.
+    intros ->. apply (Hκmin κ'). done. by apply strict_spec_alt. }
+  { intros κ' κ'' [γs'' ?].
+    destruct (decide (κ'' = κ)) as [->|]; [intros; set_solver +|].
+    intros. rewrite elem_of_union. right. apply (HK' κ'); eauto. set_solver. set_solver. }
+  { rewrite /Iinv. iFrame "HI".
+    iApply (big_sepS_insert _ K'); first done. iFrame. }
+  iDestruct (big_sepS_insert _ K' with "Halive") as "[Hκalive Halive]"; first done.
+  iMod (lft_kill with "[$HI $Halive $Hdead] Hκalive Hκ")
+    as "[(HI&Halive&Hdead) Hκdead]".
+  { intros κ' ??. eapply HK'. eauto.
+    intros ?. rewrite -> minimal_strict in Hκmin.
+    eapply (Hκmin κ'). eauto. eauto. eauto. eauto. }
+  { intros κ' ??. rewrite elem_of_difference elem_of_singleton. split.
+    2: by apply strict_spec_alt in H3 as [??].
+    eapply HK. eauto. eauto.
+     by apply strict_spec_alt in H3 as [??]. }
+  iModIntro. rewrite /Iinv. iFrame.
+  iApply (big_sepS_delete _ K). done. iFrame.
+Qed.
+
+Lemma lft_create E :
+  nclose lftN ⊆ E →
+  lft_ctx ={E}=∗ ∃ κ, 1.[κ] ∗ □ (1.[κ] ={⊤,⊤∖nclose lftN}▷=∗ [†κ]).
+Proof.
+  iIntros (?) "#Hmgmt".
+  iInv mgmtN as (A I) "(>HA & >HI & Hinv)" "Hclose".
+  destruct (exist_fresh (dom (gset _) A)) as [Λ HΛ%not_elem_of_dom].
+  iMod (own_update with "HA") as "[HA HΛ]".
+  { apply auth_update_alloc, (alloc_singleton_local_update _ Λ (Cinl 1%Qp))=>//.
+    by rewrite lookup_fmap HΛ. }
+  iMod ("Hclose" with "[HA HI Hinv]") as "_".
+  { iNext; iExists (<[Λ:=true]>A), I; rewrite fmap_insert; iFrame.
+    iApply (big_sepS_impl _ _ (dom (gset lft) I) with "[$Hinv]").
+    iAlways; iIntros (κ ?) "[[Hκ %]|[Hκ HA]]".
+    - iLeft. iFrame "Hκ". iPureIntro=> Λ' ?; rewrite lookup_insert_Some.
+      destruct (decide (Λ = Λ')); auto.
+    - iRight. iFrame "Hκ". iDestruct "HA" as %(Λ' & ? & ?).
+      iPureIntro; exists Λ'. rewrite lookup_insert_ne; last congruence. auto. }
+  iModIntro; iExists {[ Λ ]}.
+  rewrite {1}/lft_own big_sepMS_singleton. iFrame "HΛ".
+  clear I A HΛ. iIntros "!# HΛ".
+  iApply (step_fupd_mask_mono ⊤ _ _ (⊤∖nclose mgmtN)).
+  { admit. } { done. }
+  iInv mgmtN as (A I) "(>HA & >HI & Hinv)" "Hclose".
+
+  iDestruct (ilft_create with "#Hinv")
+
+  rewrite /lft_own big_sepMS_singleton.
+  iDestruct (own_valid_2 with "HA HΛ")
+    as %[[s [?%leibniz_equiv ?]]%singleton_included _]%auth_valid_discrete_2.
+  iMod (own_update_2 with "HA HΛ") as "[HA HΛ]".
+  { by eapply auth_update, singleton_local_update,
+     (exclusive_local_update _ (Cinr ())). }
+  iAssert [†{[Λ]}]%I with "[HΛ]" as "HΛ".
+  { iExists Λ. iFrame "HΛ". iPureIntro; set_solver. }
+  iModIntro; iNext.
+  set (K := filter (λ κ, Λ ∈ κ) (dom (gset lft) I)).
+  
+K ∪ {[ static ]}
+
+  iDestruct (lfts_kill I K {[ static ]} with "[$HI]") as "?".
+
+
+
+SearchAbout filter.
+
+{ I !! κ = Some κ 
+ rewrite elem_of_singetoen. set_solver. eauto. first done.
+SearchAbout included Exclusive.
+Check exclusive_local_update _ (Cinr ()).
+SearchAbout local_update singletonM. 
+
+ Check fupd_intro_mask.
+SearchAbout fupd.
+SearchAbout local_update gmap.
+ gmap_local_update_alloc .
+
+Admitted.
+
+(** Basic borrows  *)
+Lemma bor_create E κ P :
+  nclose lftN ⊆ E →
+  lft_ctx ⊢ ▷ P ={E}=∗ &{κ} P ∗ ([†κ] ={E}=∗ ▷ P).
+Proof. Admitted.
+Lemma bor_fake E κ P :
+  nclose lftN ⊆ E →
+  lft_ctx ⊢ [†κ] ={E}=∗ &{κ}P.
+Proof.
+  iIntros (?) "#?". iDestruct 1 as (Λ) "[% ?]".
+Admitted.
+Lemma bor_sep E κ P Q :
+  nclose lftN ⊆ E →
+  lft_ctx ⊢ &{κ} (P ∗ Q) ={E}=∗ &{κ} P ∗ &{κ} Q.
+Proof.
+  iIntros (?) "#? Hbor".
+Admitted.
+Lemma bor_combine E κ P Q :
+  nclose lftN ⊆ E →
+  lft_ctx ⊢ &{κ} P -∗ &{κ} Q ={E}=∗ &{κ} (P ∗ Q).
+Proof. Admitted.
+Lemma bor_acc_strong E q κ P :
+  nclose lftN ⊆ E →
+  lft_ctx ⊢ &{κ} P -∗ q.[κ] ={E}=∗ ▷ P ∗
+    ∀ Q, ▷ Q ∗ ▷([†κ] -∗ ▷ Q ={⊤∖nclose lftN}=∗ ▷ P) ={E}=∗ &{κ} Q ∗ q.[κ].
+Proof. Admitted.
+Lemma bor_acc_atomic_strong E κ P :
+  nclose lftN ⊆ E →
+  lft_ctx ⊢ &{κ} P ={E,E∖lftN}=∗
+    (▷ P ∗ ∀ Q, ▷ Q ∗ ▷ ([†κ] -∗ ▷ Q ={⊤∖nclose lftN}=∗ ▷ P) ={E∖lftN,E}=∗ &{κ} Q) ∨
+    [†κ] ∗ |={E∖lftN,E}=> True.
+Proof. Admitted.
+Lemma bor_reborrow' E κ κ' P :
+  nclose lftN ⊆ E → κ ⊆ κ' →
+  lft_ctx ⊢ &{κ} P ={E}=∗ &{κ'} P ∗ ([†κ'] ={E}=∗ &{κ} P).
+Proof. Admitted.
+Lemma bor_unnest E κ κ' P :
+  nclose lftN ⊆ E →
+  lft_ctx ⊢ &{κ'} &{κ} P ={E}▷=∗ &{κ ∪ κ'} P.
+Proof. Admitted.
+
+(** Indexed borrow *)
+Lemma idx_bor_acc E q κ i P :
+  nclose lftN ⊆ E →
+  lft_ctx ⊢ idx_bor κ i P -∗ idx_bor_own 1 i -∗ q.[κ] ={E}=∗
+            ▷ P ∗ (▷ P ={E}=∗ idx_bor_own 1 i ∗ q.[κ]).
+Proof. Admitted.
+
+Lemma idx_bor_atomic_acc E q κ i P :
+  nclose lftN ⊆ E →
+  lft_ctx ⊢ idx_bor κ i P -∗ idx_bor_own q i ={E,E∖lftN}=∗
+              ▷ P ∗ (▷ P ={E∖lftN,E}=∗ idx_bor_own q i) ∨
+              [†κ] ∗ (|={E∖lftN,E}=> idx_bor_own q i).
+Proof. Admitted.
+
+Lemma idx_bor_shorten κ κ' i P :
+  κ ⊑ κ' ⊢ idx_bor κ' i P -∗ idx_bor κ i P.
+Proof. Admitted.
 
   (*** Derived lemmas  *)
-
-  Lemma lft_own_dead q κ : q.[κ] ⊢ [† κ] -∗ False.
-  Proof.
-    rewrite /lft_own /lft_dead.
-    iIntros "Hl Hr". iDestruct "Hr" as (Λ) "[HΛ Hr]".
-    iDestruct "HΛ" as %[n HΛ].
-    iDestruct (own_valid_2 with "[$Hl $Hr]") as %Hval. iPureIntro.
-    generalize (Hval Λ).
-    by rewrite lookup_op lookup_singleton lookup_fmap lookup_omap HΛ.
-  Qed.
-
-  Lemma lft_own_static q : True ==∗ q.[static].
-  Proof.
-    rewrite /lft_own /static omap_empty fmap_empty.
-    apply (own_empty lft_tokUR lft_toks_name).
-  Qed.
-
-  Lemma lft_not_dead_static : [† static] ⊢ False.
-  Proof.
-    rewrite /lft_dead /static. setoid_rewrite lookup_empty.
-    iIntros "HΛ". iDestruct "HΛ" as (Λ) "[% _]". naive_solver.
-  Qed.
-
-  Lemma lft_own_split κ q : q.[κ] ⊣⊢ (q/2).[κ] ∗ (q/2).[κ].
-  Proof. by rewrite -lft_own_frac_op Qp_div_2. Qed.
-
-  Global Instance into_and_lft_own_half κ q :
-    IntoAnd false q.[κ] (q/2).[κ] (q/2).[κ] | 100.
-  Proof. by rewrite /IntoAnd lft_own_split. Qed.
-
-  Global Instance from_sep_lft_own_half κ q :
-    FromSep q.[κ] (q/2).[κ] (q/2).[κ] | 100.
-  Proof. by rewrite /FromSep -lft_own_split. Qed.
-
-  Global Instance frame_lft_own_half κ q :
-    Frame (q/2).[κ] q.[κ] (q/2).[κ] | 100.
-  Proof. by rewrite /Frame -lft_own_split. Qed.
-
-  Global Instance into_and_lft_own_frac κ q1 q2 :
-    IntoAnd false (q1+q2).[κ] q1.[κ] q2.[κ].
-  Proof. by rewrite /IntoAnd lft_own_frac_op. Qed.
-
-  Global Instance from_sep_lft_own_frac κ q1 q2 :
-    FromSep (q1+q2).[κ] q1.[κ] q2.[κ].
-  Proof. by rewrite /FromSep -lft_own_frac_op. Qed.
-
-  Global Instance into_and_lft_own κ1 κ2 q :
-    IntoAnd false q.[κ1⋅κ2] q.[κ1] q.[κ2].
-  Proof. by rewrite /IntoAnd lft_own_op. Qed.
-
-  Global Instance from_sep_lft_own κ1 κ2 q :
-    FromSep q.[κ1⋅κ2] q.[κ1] q.[κ2].
-  Proof. by rewrite /FromSep lft_own_op. Qed.
 
   Lemma borrow_acc E q κ P : nclose lftN ⊆ E →
       lft_ctx ⊢ &{κ}P -∗ q.[κ] ={E}=∗ ▷ P ∗ (▷ P ={E}=∗ &{κ}P ∗ q.[κ]).
@@ -256,23 +692,6 @@ Section lft.
     by iMod ("Hob" with "HP") as "[_$]".
   Qed.
 
-End lft.
-
-Typeclasses Opaque borrow.
-
-(*** Inclusion and shortening. *)
-
-Definition lft_incl `{invG Σ, lifetimeG Σ} κ κ' : iProp Σ :=
-  (□((∀ q, q.[κ] ={lftN}=∗ ∃ q', q'.[κ'] ∗ (q'.[κ'] ={lftN}=∗ q.[κ])) ∗
-     ([†κ'] ={lftN}=∗ [†κ])))%I.
-
-Infix "⊑" := lft_incl (at level 60) : C_scope.
-
-Section incl.
-  Context `{invG Σ, lifetimeG Σ}.
-
-  Global Instance lft_incl_persistent κ κ': PersistentP (κ ⊑ κ') := _.
-
   Lemma lft_incl_acc `(nclose lftN ⊆ E) κ κ' q:
     κ ⊑ κ' ⊢ q.[κ] ={E}=∗ ∃ q', q'.[κ'] ∗ (q'.[κ'] ={E}=∗ q.[κ]).
   Proof.
@@ -290,7 +709,7 @@ Section incl.
   Proof.
     iIntros ([κ0 ->%leibniz_equiv]) "!#". iSplitR.
     - iIntros (q) "[Hκ' Hκ0]". iExists q. iIntros "!>{$Hκ'}Hκ'!>". by iSplitR "Hκ0".
-    - iIntros "?!>". iApply lft_dead_or. auto.
+    - iIntros "? !>". iApply lft_dead_or. auto.
   Qed.
 
   Lemma lft_incl_refl κ : True ⊢ κ ⊑ κ.
@@ -307,8 +726,7 @@ Section incl.
     - iIntros "H†". iMod ("H2†" with "H†"). by iApply "H1†".
   Qed.
 
-  Axiom idx_borrow_shorten :
-    ∀ κ κ' i P, κ ⊑ κ' ⊢ idx_borrow κ' i P -∗ idx_borrow κ i P.
+
 
   Lemma borrow_shorten κ κ' P: κ ⊑ κ' ⊢ &{κ'}P -∗ &{κ}P.
   Proof.
